\begin{align*}
\frac{\mathrm d}{\mathrm d\tau}\frac{\partial L}{\partial v^\mu}
  -\frac{\partial L}{\partial x^\mu} &= 0\\
  L&=-mc\sqrt{v^\mu_\mu}-\frac{e}{c}v^\mu A_\mu & \tau:&=\frac{t}{\gamma}\\
  \frac{\mathrm d}{\mathrm d\frac{t}{\gamma}}\frac{\partial L}{\partial v^\mu}
  -\frac{\partial L}{\partial x^\mu} &= 0\\
  \gamma\frac{\mathrm d}{\mathrm dt}\frac{\partial L}{\partial v^\mu}
   &= \frac{\partial L}{\partial x^\mu}\\
  \gamma\frac{\mathrm d}{\mathrm dt}\frac{\partial (-mc\sqrt{v^\mu_\mu}-\frac{e}{c}v^\mu A_\mu)}{\partial v^\mu}
   &= \frac{\partial (-mc\sqrt{v^\mu_\mu}-\frac{e}{c}v^\mu A_\mu)}{\partial x^\mu}\\
  \gamma\frac{\mathrm d}{\mathrm dt}(-mc\sqrt{v^\mu_\mu}-\frac{e}{c} A_\mu)
   &= \frac{\partial (-mc\sqrt{v^\mu_\mu}-\frac{e}{c}v^\mu A_\mu)}{\partial x^\mu}\\
\end{align}
